some progress?

Impl/BookkeepingImpl.i.dfy
@@ -18,276 +18,106 @@ module BookkeepingImpl {
 
   import opened Bounds
 
-  predicate RefAvailable(s: ImplVariables, ref: BT.G.Reference)
-    requires s.Ready? && s.W()
-  {
-    && ref !in s.ephemeralIndirectionTable.I().graph
-    && ref !in s.cache.I()
-    && ref != BT.G.Root()
-  }
+  // method getFreeRef(shared s: ImplVariables)
+  // returns (ref : Option<BT.G.Reference>)
+  // requires s.Ready?
+  // requires s.W()
 
-  method getFreeRef(shared s: ImplVariables)
-  returns (ref : Option<BT.G.Reference>)
-  requires s.Ready?
-  requires s.W()
+  // ensures s.Ready?
+  // ensures s.W()
+  // ensures ref.Some? ==> s.RefAvailable(ref.value)
+  // ensures forall ref1 | ref1 in s.cache.I() :: Some(ref1) != ref
 
-  ensures s.Ready?
-  ensures s.W()
-  ensures ref.Some? ==> RefAvailable(s, ref.value)
-  ensures forall ref1 | ref1 in s.cache.I() :: Some(ref1) != ref
+  // ensures var gs := s.I();
+  //   && (forall r | r in gs.ephemeralIndirectionTable.graph :: r <= gs.ephemeralIndirectionTable.refUpperBound)
+  //   && ref == BookkeepingModel.getFreeRef(gs);
+  // {
+  //   BookkeepingModel.reveal_getFreeRef();
 
-  ensures var gs := s.I();
-    && (forall r | r in gs.ephemeralIndirectionTable.graph :: r <= gs.ephemeralIndirectionTable.refUpperBound)
-    && ref == BookkeepingModel.getFreeRef(gs);
-  {
-    BookkeepingModel.reveal_getFreeRef();
+  //   ghost var getable := s.I().ephemeralIndirectionTable;
 
-    ghost var getable := s.I().ephemeralIndirectionTable;
+  //   assert forall r | r in getable.graph :: r <= getable.refUpperBound by {
+  //     s.ephemeralIndirectionTable.UpperBounded();
+  //     assert forall r | r in s.ephemeralIndirectionTable.graph :: r <= s.ephemeralIndirectionTable.refUpperBound;
+  //   }
 
-    assert forall r | r in getable.graph :: r <= getable.refUpperBound by {
-      s.ephemeralIndirectionTable.UpperBounded();
-      assert forall r | r in s.ephemeralIndirectionTable.graph :: r <= s.ephemeralIndirectionTable.refUpperBound;
-    }
+  //   var i := s.ephemeralIndirectionTable.GetRefUpperBound();
+  //   if i == 0xffff_ffff_ffff_ffff {
+  //     return None;
+  //   }
 
-    var i := s.ephemeralIndirectionTable.GetRefUpperBound();
-    if i == 0xffff_ffff_ffff_ffff {
-      return None;
-    }
+  //   i := i + 1;
 
-    i := i + 1;
-
-    while true
-    invariant i >= 1
-    invariant forall r | r in s.ephemeralIndirectionTable.graph :: r < i
-    invariant BookkeepingModel.getFreeRefIterate(s.I(), i)
-           == BookkeepingModel.getFreeRef(s.I())
-    decreases 0x1_0000_0000_0000_0000 - i as int
-    {
-      var cacheLookup := s.cache.InCache(i);
-      if !cacheLookup {
-        return Some(i);
-      }
+  //   while true
+  //   invariant i >= 1
+  //   invariant forall r | r in s.ephemeralIndirectionTable.graph :: r < i
+  //   invariant BookkeepingModel.getFreeRefIterate(s.I(), i)
+  //          == BookkeepingModel.getFreeRef(s.I())
+  //   decreases 0x1_0000_0000_0000_0000 - i as int
+  //   {
+  //     var cacheLookup := s.cache.InCache(i);
+  //     if !cacheLookup {
+  //       return Some(i);
+  //     }
       
-      if i == 0xffff_ffff_ffff_ffff {
-        return None;
-      } else {
-        i := i + 1;
-      }
-    }
-  }
+  //     if i == 0xffff_ffff_ffff_ffff {
+  //       return None;
+  //     } else {
+  //       i := i + 1;
+  //     }
+  //   }
+  // }
 
-  method getFreeRef2(shared s: ImplVariables, avoid: BT.G.Reference)
-  returns (ref : Option<BT.G.Reference>)
-  requires s.Ready?
-  requires s.W()
+  // method getFreeRef2(shared s: ImplVariables, avoid: BT.G.Reference)
+  // returns (ref : Option<BT.G.Reference>)
+  // requires s.Ready?
+  // requires s.W()
 
-  ensures ref.Some? ==> ref.value != avoid;
-  ensures ref.Some? ==> RefAvailable(s, ref.value)
-  ensures forall ref1 | ref1 in s.cache.I() :: Some(ref1) != ref
+  // ensures ref.Some? ==> ref.value != avoid;
+  // ensures ref.Some? ==> RefAvailable(s, ref.value)
+  // ensures forall ref1 | ref1 in s.cache.I() :: Some(ref1) != ref
 
-  ensures var gs := s.I();
-    && (forall r | r in gs.ephemeralIndirectionTable.graph :: r <= gs.ephemeralIndirectionTable.refUpperBound)
-    && ref == BookkeepingModel.getFreeRef2(gs, avoid);
-  {
-    BookkeepingModel.reveal_getFreeRef2();
+  // ensures var gs := s.I();
+  //   && (forall r | r in gs.ephemeralIndirectionTable.graph :: r <= gs.ephemeralIndirectionTable.refUpperBound)
+  //   && ref == BookkeepingModel.getFreeRef2(gs, avoid);
+  // {
+  //   BookkeepingModel.reveal_getFreeRef2();
 
-    ghost var getable := s.I().ephemeralIndirectionTable;
+  //   ghost var getable := s.I().ephemeralIndirectionTable;
 
-    assert forall r | r in getable.graph :: r <= getable.refUpperBound by {
-      s.ephemeralIndirectionTable.UpperBounded();
-      assert forall r | r in s.ephemeralIndirectionTable.graph :: r <= s.ephemeralIndirectionTable.refUpperBound;
-    }
+  //   assert forall r | r in getable.graph :: r <= getable.refUpperBound by {
+  //     s.ephemeralIndirectionTable.UpperBounded();
+  //     assert forall r | r in s.ephemeralIndirectionTable.graph :: r <= s.ephemeralIndirectionTable.refUpperBound;
+  //   }
 
-    var i := s.ephemeralIndirectionTable.GetRefUpperBound();
-    if i == 0xffff_ffff_ffff_ffff {
-      return None;
-    }
+  //   var i := s.ephemeralIndirectionTable.GetRefUpperBound();
+  //   if i == 0xffff_ffff_ffff_ffff {
+  //     return None;
+  //   }
 
-    i := i + 1;
+  //   i := i + 1;
 
-    while true
-    invariant i >= 1
-    invariant forall r | r in s.ephemeralIndirectionTable.I().graph :: r < i
-    invariant BookkeepingModel.getFreeRef2Iterate(s.I(), avoid, i)
-           == BookkeepingModel.getFreeRef2(s.I(), avoid)
-    decreases 0x1_0000_0000_0000_0000 - i as int
-    {
-      if i != avoid {
-        var cacheLookup := s.cache.InCache(i);
-        if !cacheLookup {
-          return Some(i);
-        }
-      }
+  //   while true
+  //   invariant i >= 1
+  //   invariant forall r | r in s.ephemeralIndirectionTable.I().graph :: r < i
+  //   invariant BookkeepingModel.getFreeRef2Iterate(s.I(), avoid, i)
+  //          == BookkeepingModel.getFreeRef2(s.I(), avoid)
+  //   decreases 0x1_0000_0000_0000_0000 - i as int
+  //   {
+  //     if i != avoid {
+  //       var cacheLookup := s.cache.InCache(i);
+  //       if !cacheLookup {
+  //         return Some(i);
+  //       }
+  //     }
       
-      if i == 0xffff_ffff_ffff_ffff {
-        return None;
-      } else {
-        i := i + 1;
-      }
-    }
-  }
-
-  lemma lemmaIndirectionTableLocIndexValid(s: ImplVariables, ref: BT.G.Reference)
-  requires s.W()
-  requires s.WriteAllocConditions()
-  ensures ref in s.ephemeralIndirectionTable.locs ==>
-    (
-      && 0 <= s.ephemeralIndirectionTable.locs[ref].addr as int / NodeBlockSize() < NumBlocks()
-      && (s.ephemeralIndirectionTable.locs[ref].addr as int / NodeBlockSize()) * NodeBlockSize() == s.ephemeralIndirectionTable.locs[ref].addr as int
-    )
-  {
-    if ref in s.ephemeralIndirectionTable.locs {
-      reveal_ConsistentBitmapInteral();
-      var loc := s.ephemeralIndirectionTable.locs[ref];
-      var i := loc.addr as int / NodeBlockSize();
-      assert s.ephemeralIndirectionTable.I().locs[ref] == loc;
-      assert loc in s.ephemeralIndirectionTable.I().locs.Values;
-      assert DiskLayout.ValidNodeLocation(loc);
-      DiskLayout.reveal_ValidNodeAddr();
-      assert i * NodeBlockSize() == loc.addr as int;
-      assert IT.IndirectionTable.IsLocAllocBitmap(s.blockAllocator.I().ephemeral, i);
-    }
-  }
-
-  lemma freeIndirectionTableLocCorrect(
-      s: ImplVariables, s': ImplVariables, ref: BT.G.Reference, j: Option<int>)
-  requires s.WriteAllocConditions()
-  requires s.W()
-  requires s'.W()
-  requires s'.Ready?
-  requires forall r | r != ref ::
-      MapsAgreeOnKey(
-          s.ephemeralIndirectionTable.I().locs,
-          s'.ephemeralIndirectionTable.I().locs,
-          r)
-  requires ref !in s'.ephemeralIndirectionTable.I().locs
-  requires j.Some? ==> 0 <= j.value < NumBlocks()
-  requires j.Some? ==> ref in s.ephemeralIndirectionTable.I().locs
-  requires j.Some? ==> s.ephemeralIndirectionTable.I().locs[ref].addr as int == j.value * NodeBlockSize()
-  requires j.Some? ==> s'.blockAllocator.I() == BlockAllocatorModel.MarkFreeEphemeral(s.blockAllocator.I(), j.value)
-  requires j.None? ==> s'.blockAllocator == s.blockAllocator
-  requires j.None? ==> ref !in s.ephemeralIndirectionTable.I().locs
-  ensures (forall i: int :: s'.ephemeralIndirectionTable.I().IsLocAllocIndirectionTable(i)
-      <==> IT.IndirectionTable.IsLocAllocBitmap(s'.blockAllocator.I().ephemeral, i))
-  ensures BlockAllocatorModel.Inv(s'.blockAllocator.I())
-  ensures BC.AllLocationsForDifferentRefsDontOverlap(
-        s'.ephemeralIndirectionTable.I())
-  ensures (forall loc |
-        loc in s'.ephemeralIndirectionTable.I().locs.Values :: 
-          DiskLayout.ValidNodeLocation(loc))
-  {
-    reveal_ConsistentBitmapInteral();
-    BitmapModel.reveal_IsSet();
-    BitmapModel.reveal_BitUnset();
-    lemmaIndirectionTableLocIndexValid(s, ref);
-
-    forall r1, r2 | r1 in s'.ephemeralIndirectionTable.I().locs && r2 in s'.ephemeralIndirectionTable.I().locs
-    ensures BC.LocationsForDifferentRefsDontOverlap(s'.ephemeralIndirectionTable.I(), r1, r2)
-    {
-      assert MapsAgreeOnKey( s.ephemeralIndirectionTable.I().locs, s'.ephemeralIndirectionTable.I().locs, r1);
-      assert MapsAgreeOnKey( s.ephemeralIndirectionTable.I().locs, s'.ephemeralIndirectionTable.I().locs, r2);
-    }
-
-    forall loc | loc in s'.ephemeralIndirectionTable.I().locs.Values
-    ensures DiskLayout.ValidNodeLocation(loc)
-    {
-      var r :| r in s'.ephemeralIndirectionTable.I().locs && s'.ephemeralIndirectionTable.I().locs[r] == loc;
-      assert MapsAgreeOnKey(s.ephemeralIndirectionTable.I().locs, s'.ephemeralIndirectionTable.I().locs, r);
-    }
-
-    if j.Some? {
-      assert DiskLayout.ValidNodeLocation(s.ephemeralIndirectionTable.I().locs[ref]);
-      assert j.value >= MinNodeBlockIndex() by {
-        DiskLayout.reveal_ValidNodeAddr();
-      }
-    }
-
-    forall i: int
-    | s'.ephemeralIndirectionTable.I().IsLocAllocIndirectionTable(i)
-    ensures IT.IndirectionTable.IsLocAllocBitmap(s'.blockAllocator.I().ephemeral, i)
-    {
-      if j.Some? && i == j.value {
-        if 0 <= i < MinNodeBlockIndex() {
-          assert false;
-        } else {
-          var r :| r in s'.ephemeralIndirectionTable.locs &&
-              s'.ephemeralIndirectionTable.locs[r].addr as int == i * NodeBlockSize() as int;
-          assert MapsAgreeOnKey(
-            s.ephemeralIndirectionTable.I().locs,
-            s'.ephemeralIndirectionTable.I().locs, r);
-
-          assert BC.LocationsForDifferentRefsDontOverlap(s.ephemeralIndirectionTable.I(), ref, r);
-
-          assert ref !in s'.ephemeralIndirectionTable.I().locs;
-          assert r in s'.ephemeralIndirectionTable.I().locs;
-          assert s.ephemeralIndirectionTable.I().locs[r]
-              == s.ephemeralIndirectionTable.I().locs[ref];
-          assert r == ref;
-
-          assert false;
-        }
-      } else {
-        if 0 <= i < MinNodeBlockIndex() {
-          assert s.ephemeralIndirectionTable.I().IsLocAllocIndirectionTable(i);
-          assert IT.IndirectionTable.IsLocAllocBitmap(s.blockAllocator.I().ephemeral, i);
-          assert IT.IndirectionTable.IsLocAllocBitmap(s'.blockAllocator.I().ephemeral, i);
-        } else {
-          var r :| r in s'.ephemeralIndirectionTable.locs &&
-              s'.ephemeralIndirectionTable.locs[r].addr as int == i * NodeBlockSize() as int;
-          assert MapsAgreeOnKey(
-            s.ephemeralIndirectionTable.I().locs,
-            s'.ephemeralIndirectionTable.I().locs, r);
-          assert s.ephemeralIndirectionTable.I().IsLocAllocIndirectionTable(i);
-          assert IT.IndirectionTable.IsLocAllocBitmap(s.blockAllocator.I().ephemeral, i);
-          assert IT.IndirectionTable.IsLocAllocBitmap(s'.blockAllocator.I().ephemeral, i);
-        }
-      }
-    }
-
-    forall i: int
-    | IT.IndirectionTable.IsLocAllocBitmap(s'.blockAllocator.I().ephemeral, i)
-    ensures s'.ephemeralIndirectionTable.I().IsLocAllocIndirectionTable(i)
-    {
-      if j.Some? && i == j.value {
-        assert s'.ephemeralIndirectionTable.I().IsLocAllocIndirectionTable(i);
-      } else {
-        assert IT.IndirectionTable.IsLocAllocBitmap(s.blockAllocator.I().ephemeral, i);
-        assert s.ephemeralIndirectionTable.I().IsLocAllocIndirectionTable(i);
-        if 0 <= i < MinNodeBlockIndex() {
-          assert s'.ephemeralIndirectionTable.I().IsLocAllocIndirectionTable(i);
-        } else {
-          var r :| r in s.ephemeralIndirectionTable.locs &&
-            s.ephemeralIndirectionTable.locs[r].addr as int == i * NodeBlockSize() as int;
-          assert MapsAgreeOnKey(
-            s.ephemeralIndirectionTable.I().locs,
-            s'.ephemeralIndirectionTable.I().locs, r);
-          assert r in s'.ephemeralIndirectionTable.locs &&
-            s'.ephemeralIndirectionTable.locs[r].addr as int == i * NodeBlockSize() as int;
-          assert s'.ephemeralIndirectionTable.I().IsLocAllocIndirectionTable(i);
-        }
-      }
-    }
-
-    if j.Some? {
-      forall i | 0 <= i < NumBlocks()
-      ensures BitmapModel.IsSet(s'.blockAllocator.I().full, i) == (
-        || BitmapModel.IsSet(s'.blockAllocator.I().ephemeral, i)
-        || (s'.blockAllocator.I().frozen.Some? && BitmapModel.IsSet(s'.blockAllocator.I().frozen.value, i))
-        || BitmapModel.IsSet(s'.blockAllocator.I().persistent, i)
-        || BitmapModel.IsSet(s'.blockAllocator.I().full, i)
-      )
-      {
-        if i == j.value {
-        } else {
-          assert BitmapModel.IsSet(s'.blockAllocator.I().full, i) == BitmapModel.IsSet(s.blockAllocator.I().full, i);
-          assert BitmapModel.IsSet(s'.blockAllocator.I().ephemeral, i) == BitmapModel.IsSet(s.blockAllocator.I().ephemeral, i);
-          assert s'.blockAllocator.I().frozen.Some? ==> BitmapModel.IsSet(s'.blockAllocator.I().frozen.value, i) == BitmapModel.IsSet(s.blockAllocator.I().frozen.value, i);
-          assert BitmapModel.IsSet(s'.blockAllocator.I().persistent, i) == BitmapModel.IsSet(s.blockAllocator.I().persistent, i);
-          assert BitmapModel.IsSet(s'.blockAllocator.I().outstanding, i) == BitmapModel.IsSet(s.blockAllocator.I().outstanding, i);
-        }
-      }
-    }
-  }
+  //     if i == 0xffff_ffff_ffff_ffff {
+  //       return None;
+  //     } else {
+  //       i := i + 1;
+  //     }
+  //   }
+  // }
 
   method writeBookkeeping(linear inout s: ImplVariables, ref: BT.G.Reference, children: Option<seq<BT.G.Reference>>)
   requires old_s.W()
@@ -304,10 +134,10 @@ module BookkeepingImpl {
 
   ensures s.WriteAllocConditions()
   ensures s.ChildrenConditions(Some([ref]))
-  ensures s.I() == BookkeepingModel.writeBookkeeping(old_s.I(), ref, children)
   ensures s.cache == old_s.cache
+  ensures BookkeepingModel.writeBookkeeping(old_s, ref, children, s)
   {
-    lemmaIndirectionTableLocIndexValid(s, ref);
+    BookkeepingModel.lemmaIndirectionTableLocIndexValid(s, ref);
     var oldLoc := inout s.ephemeralIndirectionTable.UpdateAndRemoveLoc(ref, (if children.Some? then children.value else []));
 
     inout s.lru.Use(ref);
@@ -322,69 +152,68 @@ module BookkeepingImpl {
         <= |LruModel.I(old_s.lru.Queue())| + |{ref}|
         == |LruModel.I(old_s.lru.Queue())| + 1;
 
-    reveal BookkeepingModel.writeBookkeeping();
+    // reveal BookkeepingModel.writeBookkeeping();
 
-    freeIndirectionTableLocCorrect(old_s, s, ref,
+    BookkeepingModel.freeIndirectionTableLocCorrect(old_s, s, ref,
       if oldLoc.Some?
       then Some(oldLoc.value.addr as int / NodeBlockSize())
       else None);
     reveal_ConsistentBitmapInteral();
-    assert s.WriteAllocConditions();
   }
 
-  method allocBookkeeping(linear inout s: ImplVariables, children: Option<seq<BT.G.Reference>>)
-  returns (ref: Option<BT.G.Reference>)
-  requires old_s.W()
-  requires old_s.Ready?
-  requires |LruModel.I(old_s.lru.Queue())| <= 0x1_0000_0000
-  requires old_s.WriteAllocConditions()
-  requires old_s.ChildrenConditions(children)
-  requires |old_s.ephemeralIndirectionTable.I().graph| < IndirectionTable.MaxSize()
-  ensures s.Ready?
+  // method allocBookkeeping(linear inout s: ImplVariables, children: Option<seq<BT.G.Reference>>)
+  // returns (ref: Option<BT.G.Reference>)
+  // requires old_s.W()
+  // requires old_s.Ready?
+  // requires |LruModel.I(old_s.lru.Queue())| <= 0x1_0000_0000
+  // requires old_s.WriteAllocConditions()
+  // requires old_s.ChildrenConditions(children)
+  // requires |old_s.ephemeralIndirectionTable.I().graph| < IndirectionTable.MaxSize()
+  // ensures s.Ready?
 
-  ensures s.W()
-  ensures |LruModel.I(s.lru.Queue())| <= |LruModel.I(old_s.lru.Queue())| + 1
-  ensures s.cache.I() == old_s.cache.I()
-  ensures ref.Some? ==> s.ChildrenConditions(Some([ref.value]))
-  ensures s.WriteAllocConditions()
+  // ensures s.W()
+  // ensures |LruModel.I(s.lru.Queue())| <= |LruModel.I(old_s.lru.Queue())| + 1
+  // ensures s.cache.I() == old_s.cache.I()
+  // ensures ref.Some? ==> s.ChildrenConditions(Some([ref.value]))
+  // ensures s.WriteAllocConditions()
 
-  ensures (s.I(), ref) == BookkeepingModel.allocBookkeeping(old_s.I(), children)
-  ensures ref.None? ==> s == old_s
-  {
-    BookkeepingModel.reveal_allocBookkeeping();
+  // ensures (s.I(), ref) == BookkeepingModel.allocBookkeeping(old_s.I(), children)
+  // ensures ref.None? ==> s == old_s
+  // {
+  //   BookkeepingModel.reveal_allocBookkeeping();
     
-    ref := getFreeRef(s);
-    if (ref.Some?) {
-      writeBookkeeping(inout s, ref.value, children);
-    }
-  }
+  //   ref := getFreeRef(s);
+  //   if (ref.Some?) {
+  //     writeBookkeeping(inout s, ref.value, children);
+  //   }
+  // }
 
-  method writeBookkeepingNoSuccsUpdate(linear inout s: ImplVariables, ref: BT.G.Reference)
-  requires old_s.W()
-  requires old_s.Ready?
-  requires |LruModel.I(old_s.lru.Queue())| <= 0x1_0000_0000
-  requires old_s.WriteAllocConditions()
-  requires ref in old_s.ephemeralIndirectionTable.I().graph
-  ensures s.W()
-  ensures s.I() == BookkeepingModel.writeBookkeepingNoSuccsUpdate(old_s.I(), ref)
-  ensures |LruModel.I(s.lru.Queue())| <= |LruModel.I(old_s.lru.Queue())| + 1
-  {
-    BookkeepingModel.reveal_writeBookkeepingNoSuccsUpdate();
+  // method writeBookkeepingNoSuccsUpdate(linear inout s: ImplVariables, ref: BT.G.Reference)
+  // requires old_s.W()
+  // requires old_s.Ready?
+  // requires |LruModel.I(old_s.lru.Queue())| <= 0x1_0000_0000
+  // requires old_s.WriteAllocConditions()
+  // requires ref in old_s.ephemeralIndirectionTable.I().graph
+  // ensures s.W()
+  // ensures s.I() == BookkeepingModel.writeBookkeepingNoSuccsUpdate(old_s.I(), ref)
+  // ensures |LruModel.I(s.lru.Queue())| <= |LruModel.I(old_s.lru.Queue())| + 1
+  // {
+  //   BookkeepingModel.reveal_writeBookkeepingNoSuccsUpdate();
 
-    lemmaIndirectionTableLocIndexValid(s, ref);
+  //   lemmaIndirectionTableLocIndexValid(s, ref);
 
-    var oldLoc := inout s.ephemeralIndirectionTable.RemoveLoc(ref);
+  //   var oldLoc := inout s.ephemeralIndirectionTable.RemoveLoc(ref);
 
-    inout s.lru.Use(ref);
+  //   inout s.lru.Use(ref);
 
-    if oldLoc.Some? {
-      inout s.blockAllocator.MarkFreeEphemeral(oldLoc.value.addr / NodeBlockSizeUint64());
-    }
+  //   if oldLoc.Some? {
+  //     inout s.blockAllocator.MarkFreeEphemeral(oldLoc.value.addr / NodeBlockSizeUint64());
+  //   }
 
-    LruModel.LruUse(old_s.lru.Queue(), ref);
-    assert LruModel.I(s.lru.Queue()) == LruModel.I(old_s.lru.Queue()) + {ref};
-    assert |LruModel.I(s.lru.Queue())| == |LruModel.I(old_s.lru.Queue()) + {ref}|
-        <= |LruModel.I(old_s.lru.Queue())| + |{ref}|
-        == |LruModel.I(old_s.lru.Queue())| + 1;
-  }
+  //   LruModel.LruUse(old_s.lru.Queue(), ref);
+  //   assert LruModel.I(s.lru.Queue()) == LruModel.I(old_s.lru.Queue()) + {ref};
+  //   assert |LruModel.I(s.lru.Queue())| == |LruModel.I(old_s.lru.Queue()) + {ref}|
+  //       <= |LruModel.I(old_s.lru.Queue())| + |{ref}|
+  //       == |LruModel.I(old_s.lru.Queue())| + 1;
+  // }
 }
